src/Trans2.v
@@ -9,20 +9,33 @@ Inductive t2prog :=
   | T2Abort  (rx:t2prog)
   | T2Halt.
 
+Record t2state_persist := T2PSt {
+  T2PSDisk: storage (* main disk *)
+}.
+
+Record t2state_ephem := T2ESt {
+  T2ESProg: t2prog;
+  T2ESAltDisk: option storage (* alternative disk for transactions, if in txn *)
+}.
+
 Record t2state := T2St {
-  T2SProg: t2prog;
-  T2SDisk: storage;           (* main disk *)
-  T2SAltDisk: option storage  (* alternative disk for transactions, if in txn *)
+  T2SPersist: t2state_persist;
+  T2SEphem: t2state_ephem
 }.
 
 Inductive t2step : t2state -> t2state -> Prop :=
   | T2smHalt: forall d oad,
-    t2step (T2St T2Halt d oad)                (T2St T2Halt d oad)
+    t2step (T2St (T2PSt d) (T2ESt T2Halt oad))
+           (T2St (T2PSt d) (T2ESt T2Halt oad))
   | T2smBegin: forall d rx,
-    t2step (T2St (T2Begin rx) d None)         (T2St rx d (Some d))
+    t2step (T2St (T2PSt d) (T2ESt (T2Begin rx) None))
+           (T2St (T2PSt d) (T2ESt rx (Some d)))
   | T2smProg: forall d ad dp rx,
-    t2step (T2St (T2DProg dp rx) d (Some ad)) (T2St rx d (Some (drun dp ad)))
+    t2step (T2St (T2PSt d) (T2ESt (T2DProg dp rx) (Some ad)))
+           (T2St (T2PSt d) (T2ESt rx (Some (drun dp ad))))
   | T2smCommit: forall d ad rx,
-    t2step (T2St (T2Commit rx) d (Some ad))   (T2St rx ad None)
+    t2step (T2St (T2PSt d) (T2ESt (T2Commit rx) (Some ad)))
+           (T2St (T2PSt ad) (T2ESt rx None))
   | T2smAbort: forall d ad rx,
-    t2step (T2St (T2Abort rx) d (Some ad))    (T2St rx d None).
+    t2step (T2St (T2PSt d) (T2ESt (T2Abort rx) (Some ad)))
+           (T2St (T2PSt d) (T2ESt rx None)).
